theories/zoo/proofmode.v
@@ -24,6 +24,14 @@ Implicit Types e : expr.
 Implicit Types v : val.
 Implicit Types K : ectx.
 
+#[global] Instance bi_intuitionistically_if_timeless {PROP : bi} (P : PROP) p :
+  Timeless (emp : PROP) →
+  Timeless P →
+  Timeless (□?p P).
+Proof.
+  destruct p => /= HP; apply _.
+Qed.
+
 Section zoo_G.
   Context `{zoo_G : !ZooG Σ}.
 
@@ -45,8 +53,9 @@ Section zoo_G.
     envs_entails Δ (WP (fill K e1) ∷ tid @ E {{ Φ }}).
   Proof.
     rewrite envs_entails_unseal => Hexec Hϕ HΔ HΔ'.
-    pose proof @pure_exec_fill. rewrite -wp_pure_step_later //.
     rewrite into_laterN_env_sound HΔ'.
+    pose proof pure_exec_fill.
+    rewrite -wp_pure_step //.
     iSteps.
   Qed.
   #[local] Lemma tac_wp_pure_credits' n Δ Δ' id K e1 e2 ϕ tid E Φ :
@@ -68,10 +77,11 @@ Section zoo_G.
   Proof.
     rewrite envs_entails_unseal => Hn Hexec Hϕ HΔ HΔ''.
     destruct (envs_app _ _ _) as [Δ'' |] eqn:HΔ'; last done.
-    pose proof @pure_exec_fill. rewrite -wp_pure_step_later //= Nat.add_0_r.
-    rewrite (bi.wand_entails _ _ (lc_weaken n _)) //.
     rewrite into_laterN_env_sound envs_app_sound //= HΔ''.
-    iSteps.
+    pose proof pure_exec_fill.
+    rewrite -wp_pure_step //.
+    iStep 4 as "H£".
+    iDestruct (lc_weaken with "H£") as "$"; first lia.
   Qed.
   Lemma tac_wp_pure_credits Δ Δ' id K e1 e2 ϕ tid E Φ :
     PureExec ϕ 1 e1 e2 →
@@ -109,6 +119,71 @@ Section zoo_G.
   Proof.
     apply tac_wp_pure_credits'.
     pose proof later_constant_lb. lia.
+  Qed.
+  Lemma tac_wp_pure_steps_lb Δ Δ' id p ns K e1 e2 ϕ tid E Φ :
+    PureExec ϕ 1 e1 e2 →
+    ϕ →
+    MaybeIntoLaterNEnvs 1 Δ Δ' →
+    envs_lookup id Δ' = Some (p, ⧖ ns)%I →
+    match
+      envs_simple_replace id p (Esnoc Enil
+        id (⧖ (S ns))
+      ) Δ'
+    with
+    | Some Δ'' =>
+        envs_entails Δ'' (WP fill K e2 ∷ tid @ E {{ Φ }})
+    | None =>
+        False
+    end →
+    envs_entails Δ (WP (fill K e1) ∷ tid @ E {{ Φ }}).
+  Proof.
+    rewrite envs_entails_unseal => Hexec Hϕ HΔ Hlookup HΔ'.
+    destruct (envs_simple_replace _ _ _ _) as [Δ'' |] eqn:HΔ''; last done.
+    rewrite into_laterN_env_sound envs_simple_replace_sound //= HΔ'.
+    rewrite bi.intuitionistically_if_elim.
+    iIntros "(>H⧖ & H)".
+    pose proof pure_exec_fill.
+    iApply (wp_pure_step_strong with "H⧖"); first done.
+    rewrite Nat.add_1_r. iSteps.
+    destruct p; iFrame "#∗".
+  Qed.
+  Lemma tac_wp_pure_steps_lb_credits Δ Δ' id1 p ns id2 K e1 e2 ϕ tid E Φ :
+    PureExec ϕ 1 e1 e2 →
+    ϕ →
+    MaybeIntoLaterNEnvs 1 Δ Δ' →
+    envs_lookup id1 Δ' = Some (p, ⧖ ns)%I →
+    match
+      envs_simple_replace id1 p (Esnoc Enil
+        id1 (⧖ (S ns))
+      ) Δ'
+    with
+    | Some Δ'' =>
+        match
+          envs_app false (Esnoc Enil
+            id2 (£ (later_function ns)))
+            Δ''
+        with
+        | Some Δ''' =>
+            envs_entails Δ''' (WP fill K e2 ∷ tid @ E {{ Φ }})
+        | None =>
+            False
+        end
+    | None =>
+        False
+    end →
+    envs_entails Δ (WP (fill K e1) ∷ tid @ E {{ Φ }}).
+  Proof.
+    rewrite envs_entails_unseal => Hexec Hϕ HΔ Hlookup HΔ'.
+    destruct (envs_simple_replace _ _ _ _) as [Δ'' |] eqn:HΔ''; last done.
+    rewrite into_laterN_env_sound envs_simple_replace_sound //=.
+    destruct (envs_app _ _ _) as [Δ''' |] eqn:HΔ'''; last done.
+    rewrite envs_app_sound //= HΔ'.
+    rewrite bi.intuitionistically_if_elim.
+    iIntros "(>H⧖ & H)".
+    pose proof pure_exec_fill.
+    iApply (wp_pure_step_strong with "H⧖"); first done.
+    rewrite /= Nat.add_1_r Nat.add_0_r. iStep 4.
+    destruct p; iFrame "#∗".
   Qed.
 
   Lemma tac_wp_value_nofupd Δ v tid E Φ :
@@ -320,8 +395,8 @@ Section zoo_G.
     envs_lookup id Δ' = Some (false, (l +ₗ fld) ↦ w)%I →
     match
       envs_simple_replace id false (Esnoc Enil
-      id ((l +ₗ fld) ↦ v)
-      ) Δ'
+        id ((l +ₗ fld) ↦ v))
+        Δ'
     with
     | Some Δ'' =>
         envs_entails Δ'' (WP fill K () ∷ tid @ E {{ Φ }})
@@ -490,7 +565,8 @@ Tactic Notation "wp_pures" :=
   [ progress repeat (wp_pure _; [])
   | wp_finish
   ].
-Tactic Notation "wp_pure" open_constr(e_foc) "credits:" constr(Hcredit) :=
+
+Tactic Notation "wp_pure" open_constr(e_foc) "credits:" constr(Hcredits) :=
   wp_start ltac:(fun e =>
     let Htmp := iFresh in
     let e := eval simpl in e in
@@ -502,18 +578,18 @@ Tactic Notation "wp_pure" open_constr(e_foc) "credits:" constr(Hcredit) :=
       | tc_solve
       | pm_reduce;
         first
-        [ iDestructHyp Htmp as Hcredit
-        | fail 2 "wp_pure:" Hcredit "is not fresh"
+        [ iDestructHyp Htmp as Hcredits
+        | fail 2 "wp_pure:" Hcredits "is not fresh"
         ];
         wp_finish
       ]
     )
     || fail "wp_pure: cannot find" e_foc "in" e "or" e_foc "is not a redex"
   ).
-Tactic Notation "wp_pure" "credits:" constr(Hcredit) :=
-  wp_pure _ credits:Hcredit.
-Tactic Notation "wp_pures" "credits:" constr(Hcredit) :=
-  wp_pure credits:Hcredit;
+Tactic Notation "wp_pure" "credits:" constr(Hcredits) :=
+  wp_pure _ credits:Hcredits.
+Tactic Notation "wp_pures" "credits:" constr(Hcredits) :=
+  wp_pure credits:Hcredits;
   wp_pures.
 Tactic Notation "wp_pure" open_constr(e_foc) "credit:" constr(Hcredit) :=
   wp_start ltac:(fun e =>
@@ -541,6 +617,65 @@ Tactic Notation "wp_pures" "credit:" constr(Hcredit) :=
   wp_pure credit:Hcredit;
   wp_pures.
 
+Tactic Notation "wp_pure" open_constr(e_foc) "steps:" constr(Hsteps_lb) :=
+  wp_start ltac:(fun e =>
+    let e := eval simpl in e in
+    first
+    [ reshape_expr e ltac:(fun K e' =>
+        unify e' e_foc;
+        eapply (tac_wp_pure_steps_lb _ _ (INamed Hsteps_lb) _ _ K e');
+        [ tc_solve
+        | solve_pure_exec_obligation
+        | tc_solve
+        | first
+          [ iAssumptionCore
+          | fail 3 "wp_pure:" Hsteps_lb "must provide time receipts (⧖ _)"
+          ]
+        | pm_reduce;
+          wp_finish
+        ]
+      )
+    | fail 1 "wp_pure: cannot find" e_foc "in" e "or" e_foc "is not a redex"
+    ]
+  ).
+Tactic Notation "wp_pure" "steps:" constr(Hsteps_lb) :=
+  wp_pure _ steps:Hsteps_lb.
+Tactic Notation "wp_pures" "steps:" constr(Hsteps_lb) :=
+  wp_pure steps:Hsteps_lb;
+  wp_pures.
+
+Tactic Notation "wp_pure" open_constr(e_foc) "steps:" constr(Hsteps_lb) "credits:" constr(Hcredits) :=
+  wp_start ltac:(fun e =>
+    let Htmp := iFresh in
+    let e := eval simpl in e in
+    first
+    [ reshape_expr e ltac:(fun K e' =>
+        unify e' e_foc;
+        eapply (tac_wp_pure_steps_lb_credits _ _ (INamed Hsteps_lb) _ _ Htmp K e');
+        [ tc_solve
+        | solve_pure_exec_obligation
+        | tc_solve
+        | first
+          [ iAssumptionCore
+          | fail 3 "wp_pure:" Hsteps_lb "must provide time receipts (⧖ _)"
+          ]
+        | pm_reduce;
+          first
+          [ iDestructHyp Htmp as Hcredits
+          | fail 3 "wp_pure:" Hcredits "is not fresh"
+          ];
+          wp_finish
+        ]
+      )
+    | fail 1 "wp_pure: cannot find" e_foc "in" e "or" e_foc "is not a redex"
+    ]
+  ).
+Tactic Notation "wp_pure" "steps:" constr(Hsteps_lb) "credits:" constr(Hcredits) :=
+  wp_pure _ steps:Hsteps_lb credits:Hcredits.
+Tactic Notation "wp_pures" "steps:" constr(Hsteps_lb) "credits:" constr(Hcredits) :=
+  wp_pure steps:Hsteps_lb credits:Hcredits;
+  wp_pures.
+
 #[local] Ltac wp_rec_aux tac :=
   let H1 := fresh in
   assert (H1 := ValRec_as_ValRec);
@@ -552,13 +687,21 @@ Tactic Notation "wp_rec" :=
   wp_rec_aux ltac:(fun _ =>
     wp_pure (App _ _)
   ).
-Tactic Notation "wp_rec" "credits:" constr(Hcredit) :=
+Tactic Notation "wp_rec" "credits:" constr(Hcredits) :=
   wp_rec_aux ltac:(fun _ =>
-    wp_pure (App _ _) credits:Hcredit
+    wp_pure (App _ _) credits:Hcredits
   ).
 Tactic Notation "wp_rec" "credit:" constr(Hcredit) :=
   wp_rec_aux ltac:(fun _ =>
     wp_pure (App _ _) credit:Hcredit
+  ).
+Tactic Notation "wp_rec" "steps:" constr(Hsteps_lb) :=
+  wp_rec_aux ltac:(fun _ =>
+    wp_pure (App _ _) steps:Hsteps_lb
+  ).
+Tactic Notation "wp_rec" "steps:" constr(Hsteps_lb) "credits:" constr(Hcredits) :=
+  wp_rec_aux ltac:(fun _ =>
+    wp_pure (App _ _) steps:Hsteps_lb credits:Hcredits
   ).
 
 Tactic Notation "wp_for" :=
